memmgr/malloc.h
@@ -8,11 +8,13 @@ in order to achieve the alignment.  The chunk size is at least the size
 given as argument to malloc.
 */
 
+/* TODO WASTE and ALIGN probably not needed here */ 
+
 enum {WORD = sizeof(size_t)};
 
 enum {ALIGN = 2};
 
-enum {WASTE = WORD*ALIGN - WORD};  
+enum {WASTE = WORD*ALIGN - WORD}; 
 
 enum {BIGBLOCK = (2<<16)*WORD};
 
