memmgr/malloc.v
@@ -778,25 +778,25 @@ Definition global_definitions : list (ident * globdef fundef type) :=
  (_free, Gfun(Internal f_free)) :: (_malloc, Gfun(Internal f_malloc)) :: nil).
 
 Definition public_idents : list ident :=
-(_malloc :: _free :: _fill_bin :: _pre_fill :: _size2bin :: _mmap0 ::
- _munmap :: ___builtin_debug :: ___builtin_nop ::
- ___builtin_write32_reversed :: ___builtin_write16_reversed ::
- ___builtin_read32_reversed :: ___builtin_read16_reversed ::
- ___builtin_fnmsub :: ___builtin_fnmadd :: ___builtin_fmsub ::
- ___builtin_fmadd :: ___builtin_fmin :: ___builtin_fmax ::
- ___builtin_ctzll :: ___builtin_ctzl :: ___builtin_ctz :: ___builtin_clzll ::
- ___builtin_clzl :: ___builtin_clz :: ___builtin_bswap64 ::
- ___compcert_i64_umulh :: ___compcert_i64_smulh :: ___compcert_i64_sar ::
- ___compcert_i64_shr :: ___compcert_i64_shl :: ___compcert_i64_umod ::
- ___compcert_i64_smod :: ___compcert_i64_udiv :: ___compcert_i64_sdiv ::
- ___compcert_i64_utof :: ___compcert_i64_stof :: ___compcert_i64_utod ::
- ___compcert_i64_stod :: ___compcert_i64_dtou :: ___compcert_i64_dtos ::
- ___compcert_va_composite :: ___compcert_va_float64 ::
- ___compcert_va_int64 :: ___compcert_va_int32 :: ___builtin_va_end ::
- ___builtin_va_copy :: ___builtin_va_arg :: ___builtin_va_start ::
- ___builtin_membar :: ___builtin_annot_intval :: ___builtin_annot ::
- ___builtin_memcpy_aligned :: ___builtin_fsqrt :: ___builtin_fabs ::
- ___builtin_bswap16 :: ___builtin_bswap32 :: ___builtin_bswap :: nil).
+(_malloc :: _free :: _pre_fill :: _mmap0 :: _munmap :: ___builtin_debug ::
+ ___builtin_nop :: ___builtin_write32_reversed ::
+ ___builtin_write16_reversed :: ___builtin_read32_reversed ::
+ ___builtin_read16_reversed :: ___builtin_fnmsub :: ___builtin_fnmadd ::
+ ___builtin_fmsub :: ___builtin_fmadd :: ___builtin_fmin ::
+ ___builtin_fmax :: ___builtin_ctzll :: ___builtin_ctzl :: ___builtin_ctz ::
+ ___builtin_clzll :: ___builtin_clzl :: ___builtin_clz ::
+ ___builtin_bswap64 :: ___compcert_i64_umulh :: ___compcert_i64_smulh ::
+ ___compcert_i64_sar :: ___compcert_i64_shr :: ___compcert_i64_shl ::
+ ___compcert_i64_umod :: ___compcert_i64_smod :: ___compcert_i64_udiv ::
+ ___compcert_i64_sdiv :: ___compcert_i64_utof :: ___compcert_i64_stof ::
+ ___compcert_i64_utod :: ___compcert_i64_stod :: ___compcert_i64_dtou ::
+ ___compcert_i64_dtos :: ___compcert_va_composite ::
+ ___compcert_va_float64 :: ___compcert_va_int64 :: ___compcert_va_int32 ::
+ ___builtin_va_end :: ___builtin_va_copy :: ___builtin_va_arg ::
+ ___builtin_va_start :: ___builtin_membar :: ___builtin_annot_intval ::
+ ___builtin_annot :: ___builtin_memcpy_aligned :: ___builtin_fsqrt ::
+ ___builtin_fabs :: ___builtin_bswap16 :: ___builtin_bswap32 ::
+ ___builtin_bswap :: nil).
 
 Definition prog : Clight.program := 
   mkprogram composites global_definitions public_idents _main Logic.I.
